scripts/audit_axioms.lean
@@ -1147,3 +1147,6 @@ open UOR.Bridge.F1Square
 #print axioms Analysis.eight_n_three_e
 #print axioms Analysis.nine3w_8m3d
 #print axioms Analysis.nine3w_M2
+#print axioms Analysis.nine3w_qcomp1
+#print axioms Analysis.nine3w_de
+#print axioms Analysis.qcomp_den
